src/formal/CommandoMain.lean
@@ -1,0 +1,3 @@
+import CommandoData
+
+def main : IO Unit := commandoMain
