src/formal/SidgenMain.lean
@@ -1,0 +1,3 @@
+import Codegen
+
+def main : IO Unit := sidgenMain
